<?xml version="1.0"?>
<rdf:RDF xmlns="http://purl.org/spar/pro/"
     xml:base="http://purl.org/spar/pro/"
     xmlns:tvc="http://www.essepuntato.it/2012/04/tvc/"
     xmlns:owl="http://www.w3.org/2002/07/owl#"
     xmlns:cpannotationschema="http://www.ontologydesignpatterns.org/schemas/cpannotationschema.owl#"
     xmlns:xsd="http://www.w3.org/2001/XMLSchema#"
     xmlns:skos="http://www.w3.org/2004/02/skos/core#"
     xmlns:rdfs="http://www.w3.org/2000/01/rdf-schema#"
     xmlns:rdf="http://www.w3.org/1999/02/22-rdf-syntax-ns#"
     xmlns:terms="http://purl.org/dc/terms/"
     xmlns:ti="http://www.ontologydesignpatterns.org/cp/owl/timeinterval.owl#"
     xmlns:sw-vocab-status="http://www.w3.org/2003/06/sw-vocab-status/"
     xmlns:xml="http://www.w3.org/XML/1998/namespace"
     xmlns:tisit="http://www.ontologydesignpatterns.org/cp/owl/timeindexedsituation.owl#"
     xmlns:foaf="http://xmlns.com/foaf/0.1/"
     xmlns:dc="http://purl.org/dc/elements/1.1/">
    <owl:Ontology rdf:about="http://purl.org/spar/pro/">
        <owl:imports rdf:resource="http://purl.org/swan/2.0/foaf-essential/"/>
        <owl:imports rdf:resource="http://www.essepuntato.it/2012/04/tvc"/>
        <owl:versionIRI rdf:resource="http://purl.org/spar/pro/2017-09-04"/>
        <owl:priorVersion rdf:resource="https://svn.code.sf.net/p/sempublishing/code/PRO/2017-09-04-pro-1_5_4.owl"/>
        <rdfs:comment xml:lang="en">This ontology is available at http://purl.org/spar/pro, and uses the namespace prefix pro.</rdfs:comment>
        <dc:creator rdf:datatype="http://www.w3.org/2001/XMLSchema#string">Silvio Peroni</dc:creator>
        <dc:creator rdf:datatype="http://www.w3.org/2001/XMLSchema#string">David Shotton</dc:creator>
        <dc:description xml:lang="en">PRO, the Publishing Roles Ontology, is an ontology written in OWL 2 DL for the characterization of the roles of agents (people, corporate bodies and computational agents) in the publication process.  It permits one to specify how an agent has a role relating to a contextual entity, and the period of time during which that role is held.

It is based on the Time-indexed Value in Context (TVC) ontology pattern (http://www.essepuntato.it/2012/04/tvc).

It is easy to extend the set of specified roles, simply by adding new individuals to the class pro:PublishingRole.

This ontology is imported into SCoRO, the Scholarly Contribution and Roles Ontology (http://purl.org/spar/scoro/), where it is used similarly to enable the description of a wider range of contributions and roles relating to other scholarly activities and entities, including academic administration, funded projects, research investigations, data and authorship, and to define their temporal extents and contexts, as for publishing roles in PRO.</dc:description>
        <dc:date rdf:datatype="http://www.w3.org/2001/XMLSchema#string">2017-09-04</dc:date>
        <dc:description xml:lang="en">Since roles have contexts and times that are important to take into account (for example, a person can be author of one paper and reviewer of another, while another person will be editor of a journal only for a defined period, not for ever), the PRO ontology permit these contexts to be specified, using an ontological design pattern called the time-indexed value in context (TVC) (http://www.essepuntato.it/2012/04/tvc/) which is imported into PRO. 
 
This ontology design pattern permits one to construct the following RDF statements:
       foaf:Agent pro:holdsRoleInTime [ a pro:RoleInTime pro:withRole pro:editor ] .

Thus the domain of pro:withRole is not foaf:Agent, but rather an anonymous member of the class pro:RoleInTime, which itself is the range of the property pro:holdsRoleInTime, for which the domain is foaf:Agent. 

The range of pro:withRole is the class pro:Role, whose members permit specific roles to be specified.  
   
This single step of indirection permits other contextual and temporal attributes (not shown here) to be specified for this member of the class pro:RoleInTime, putting that role into context.

Exemplar usage: 

 foaf:Agent pro:holdsRoleInTime [ a pro:RoleInTime pro:withRole pro:editor ] .</dc:description>
        <owl:versionInfo rdf:datatype="http://www.w3.org/2001/XMLSchema#string">1.5.4</owl:versionInfo>
        <rdfs:comment xml:lang="en">PRO, the Publishing Roles Ontology, is an ontology for describing roles in the publication process, or in other scholarly activities or situations, held by particular agent.  The role can be specified to exist over a defined period of time, and within a specific context, e.g. with respect to a particular document. 

PRO forms part of SPAR, a suite of Semantic Publishing and Referencing Ontologies.  Other SPAR ontologies are described at http://purl.org/spar/.</rdfs:comment>
        <dc:rights xml:lang="en">This work is distributed under a Creative Commons Attribution License (http://creativecommons.org/licenses/by/3.0/).</dc:rights>
        <dc:description rdf:resource="http://sempublishing.svn.sourceforge.net/svnroot/sempublishing/PRO/pro.png"/>
        <dc:title xml:lang="en">PRO, the Publishing Roles Ontology</dc:title>
    </owl:Ontology>
    


    <!-- 
    ///////////////////////////////////////////////////////////////////////////////////////
    //
    // Annotation properties
    //
    ///////////////////////////////////////////////////////////////////////////////////////
     -->

    


    <!-- http://purl.org/dc/elements/1.1/creator -->

    <owl:AnnotationProperty rdf:about="http://purl.org/dc/elements/1.1/creator"/>
    


    <!-- http://purl.org/dc/elements/1.1/date -->

    <owl:AnnotationProperty rdf:about="http://purl.org/dc/elements/1.1/date"/>
    


    <!-- http://purl.org/dc/elements/1.1/description -->

    <owl:AnnotationProperty rdf:about="http://purl.org/dc/elements/1.1/description"/>
    


    <!-- http://purl.org/dc/elements/1.1/rights -->

    <owl:AnnotationProperty rdf:about="http://purl.org/dc/elements/1.1/rights"/>
    


    <!-- http://purl.org/dc/elements/1.1/title -->

    <owl:AnnotationProperty rdf:about="http://purl.org/dc/elements/1.1/title"/>
    


    <!-- http://www.w3.org/2000/01/rdf-schema#comment -->

    <owl:AnnotationProperty rdf:about="http://www.w3.org/2000/01/rdf-schema#comment"/>
    


    <!-- http://www.w3.org/2000/01/rdf-schema#label -->

    <owl:AnnotationProperty rdf:about="http://www.w3.org/2000/01/rdf-schema#label"/>
    


    <!-- http://www.w3.org/2000/01/rdf-schema#seeAlso -->

    <owl:AnnotationProperty rdf:about="http://www.w3.org/2000/01/rdf-schema#seeAlso"/>
    


    <!-- http://www.w3.org/2002/07/owl#versionInfo -->

    <owl:AnnotationProperty rdf:about="http://www.w3.org/2002/07/owl#versionInfo"/>
    


    <!-- 
    ///////////////////////////////////////////////////////////////////////////////////////
    //
    // Object Properties
    //
    ///////////////////////////////////////////////////////////////////////////////////////
     -->

    


    <!-- http://purl.org/spar/pro/holdsRoleInTime -->

    <owl:ObjectProperty rdf:about="http://purl.org/spar/pro/holdsRoleInTime">
        <rdfs:subPropertyOf rdf:resource="http://www.essepuntato.it/2012/04/tvc/hasValue"/>
        <owl:inverseOf rdf:resource="http://purl.org/spar/pro/isHeldBy"/>
        <rdfs:domain rdf:resource="http://xmlns.com/foaf/0.1/Agent"/>
        <rdfs:range rdf:resource="http://purl.org/spar/pro/RoleInTime"/>
        <rdfs:comment xml:lang="en">A property relating an agent to a role that the agent holds.  This is done via the indirection: foaf:Agent pro:holdsRoleInTime [ a pro:RoleInTime ; pro:withRole pro:Role ] .  The ontology permits one to specify the time period over which a role is held, and the other contextual entities to which that agent&apos;s role relates.</rdfs:comment>
        <rdfs:label xml:lang="en">holds role in time</rdfs:label>
    </owl:ObjectProperty>
    


    <!-- http://purl.org/spar/pro/isDocumentContextFor -->

    <owl:ObjectProperty rdf:about="http://purl.org/spar/pro/isDocumentContextFor">
        <rdfs:subPropertyOf rdf:resource="http://purl.org/spar/pro/isRelatedToRoleInTime"/>
        <owl:inverseOf rdf:resource="http://purl.org/spar/pro/relatesToDocument"/>
        <rdfs:domain rdf:resource="http://xmlns.com/foaf/0.1/Document"/>
        <rdfs:comment xml:lang="en">A property relating a document to the role for which that document provides the context (e.g. relating a document to the role of author or peer-reviewer of that document).</rdfs:comment>
        <rdfs:label xml:lang="en">is document context for</rdfs:label>
    </owl:ObjectProperty>
    


    <!-- http://purl.org/spar/pro/isHeldBy -->

    <owl:ObjectProperty rdf:about="http://purl.org/spar/pro/isHeldBy">
        <rdfs:subPropertyOf rdf:resource="http://www.ontologydesignpatterns.org/cp/owl/timeindexedsituation.owl#forEntity"/>
        <rdfs:domain rdf:resource="http://purl.org/spar/pro/RoleInTime"/>
        <rdfs:range rdf:resource="http://xmlns.com/foaf/0.1/Agent"/>
        <rdfs:comment xml:lang="en">A property relating a role in time that an agent holds, or a contribution situation that an agent makes, to that agent.</rdfs:comment>
        <rdfs:label xml:lang="en">is role held by</rdfs:label>
    </owl:ObjectProperty>
    


    <!-- http://purl.org/spar/pro/isOrganizationContextFor -->

    <owl:ObjectProperty rdf:about="http://purl.org/spar/pro/isOrganizationContextFor">
        <rdfs:subPropertyOf rdf:resource="http://purl.org/spar/pro/isRelatedToRoleInTime"/>
        <owl:inverseOf rdf:resource="http://purl.org/spar/pro/relatesToOrganization"/>
        <rdfs:domain rdf:resource="http://xmlns.com/foaf/0.1/Organization"/>
        <rdfs:comment xml:lang="en">A property relating an organization to the role for which that organization provides the context (e.g. relating an institution to the role of member held by a person).</rdfs:comment>
        <rdfs:label xml:lang="it">is organization context for</rdfs:label>
    </owl:ObjectProperty>
    


    <!-- http://purl.org/spar/pro/isPersonContextFor -->

    <owl:ObjectProperty rdf:about="http://purl.org/spar/pro/isPersonContextFor">
        <rdfs:subPropertyOf rdf:resource="http://purl.org/spar/pro/isRelatedToRoleInTime"/>
        <rdfs:comment xml:lang="en">A property relating a person to the role for which that person provides the context (e.g. relating a graduate student to the role of supervisor held by a faculty member).</rdfs:comment>
        <rdfs:label xml:lang="en">is person context for</rdfs:label>
    </owl:ObjectProperty>
    


    <!-- http://purl.org/spar/pro/isRelatedToRoleInTime -->

    <owl:ObjectProperty rdf:about="http://purl.org/spar/pro/isRelatedToRoleInTime">
        <rdfs:subPropertyOf rdf:resource="http://www.ontologydesignpatterns.org/cp/owl/timeindexedsituation.owl#hasTimeIndexedSetting"/>
        <owl:inverseOf rdf:resource="http://purl.org/spar/pro/relatesToEntity"/>
        <rdfs:range rdf:resource="http://purl.org/spar/pro/RoleInTime"/>
        <rdfs:comment xml:lang="en">A property relating an entity to the role for which that entity provides the context.</rdfs:comment>
        <rdfs:label xml:lang="en">is related to role in time</rdfs:label>
    </owl:ObjectProperty>
    


    <!-- http://purl.org/spar/pro/isRoleIn -->

    <owl:ObjectProperty rdf:about="http://purl.org/spar/pro/isRoleIn">
        <rdfs:subPropertyOf rdf:resource="http://www.ontologydesignpatterns.org/cp/owl/timeindexedsituation.owl#hasTimeIndexedSetting"/>
        <owl:inverseOf rdf:resource="http://purl.org/spar/pro/withRole"/>
        <rdfs:domain rdf:resource="http://purl.org/spar/pro/Role"/>
        <rdfs:range rdf:resource="http://purl.org/spar/pro/RoleInTime"/>
        <rdfs:comment xml:lang="en">The property relating the definition of a specific role to the situation of an agent holding that role.</rdfs:comment>
        <rdfs:label xml:lang="en">is role in</rdfs:label>
    </owl:ObjectProperty>
    


    <!-- http://purl.org/spar/pro/relatesToDocument -->

    <owl:ObjectProperty rdf:about="http://purl.org/spar/pro/relatesToDocument">
        <rdfs:subPropertyOf rdf:resource="http://purl.org/spar/pro/relatesToEntity"/>
        <rdfs:range rdf:resource="http://xmlns.com/foaf/0.1/Document"/>
        <rdfs:comment xml:lang="en">A property relating a time-indexed situation describing a publishing role to a document that represents the context for that situation (e.g. relating the role of editor or peer-reviewer to the document being edited or peer-reviewed).</rdfs:comment>
        <rdfs:label xml:lang="en">relates to document</rdfs:label>
    </owl:ObjectProperty>
    


    <!-- http://purl.org/spar/pro/relatesToEntity -->

    <owl:ObjectProperty rdf:about="http://purl.org/spar/pro/relatesToEntity">
        <rdfs:subPropertyOf rdf:resource="http://www.essepuntato.it/2012/04/tvc/withinContext"/>
        <rdfs:domain rdf:resource="http://purl.org/spar/pro/RoleInTime"/>
        <rdfs:comment xml:lang="en">A property relating a time-indexed situation to an entity representing the context for that situation.</rdfs:comment>
        <rdfs:label xml:lang="en">relates to</rdfs:label>
    </owl:ObjectProperty>
    


    <!-- http://purl.org/spar/pro/relatesToOrganization -->

    <owl:ObjectProperty rdf:about="http://purl.org/spar/pro/relatesToOrganization">
        <rdfs:subPropertyOf rdf:resource="http://purl.org/spar/pro/relatesToEntity"/>
        <rdfs:range rdf:resource="http://xmlns.com/foaf/0.1/Organization"/>
        <rdfs:comment xml:lang="en">A property relating a time-indexed situation to an organization that represents the context for that situation (e.g. relating the role of member to the institution of which that person is a member).</rdfs:comment>
        <rdfs:label xml:lang="en">relates to organization</rdfs:label>
    </owl:ObjectProperty>
    


    <!-- http://purl.org/spar/pro/relatesToPerson -->

    <owl:ObjectProperty rdf:about="http://purl.org/spar/pro/relatesToPerson">
        <rdfs:subPropertyOf rdf:resource="http://purl.org/spar/pro/relatesToEntity"/>
        <rdfs:range rdf:resource="http://xmlns.com/foaf/0.1/Person"/>
        <rdfs:comment xml:lang="en">A property relating a time-indexed situation to a person who represents the context for that situation (e.g. relating the role of an supervisor with respect to the graduate student being supervised).</rdfs:comment>
        <rdfs:label xml:lang="en">relates to person</rdfs:label>
    </owl:ObjectProperty>
    


    <!-- http://purl.org/spar/pro/withRole -->

    <owl:ObjectProperty rdf:about="http://purl.org/spar/pro/withRole">
        <rdfs:subPropertyOf rdf:resource="http://www.essepuntato.it/2012/04/tvc/withValue"/>
        <rdf:type rdf:resource="http://www.w3.org/2002/07/owl#FunctionalProperty"/>
        <rdfs:domain rdf:resource="http://purl.org/spar/pro/RoleInTime"/>
        <rdfs:range rdf:resource="http://purl.org/spar/pro/Role"/>
        <rdfs:comment xml:lang="en">An object property connecting an agent&apos;s role in time to a definition of the type of role held by this agent, specified as an instance of the class pro:Role or of one of its sub-classes.</rdfs:comment>
        <rdfs:label xml:lang="en">with role</rdfs:label>
    </owl:ObjectProperty>
    


    <!-- http://www.essepuntato.it/2012/04/tvc/atTime -->

    <owl:ObjectProperty rdf:about="http://www.essepuntato.it/2012/04/tvc/atTime"/>
    


    <!-- http://www.essepuntato.it/2012/04/tvc/hasValue -->

    <owl:ObjectProperty rdf:about="http://www.essepuntato.it/2012/04/tvc/hasValue"/>
    


    <!-- http://www.essepuntato.it/2012/04/tvc/withValue -->

    <owl:ObjectProperty rdf:about="http://www.essepuntato.it/2012/04/tvc/withValue"/>
    


    <!-- http://www.essepuntato.it/2012/04/tvc/withinContext -->

    <owl:ObjectProperty rdf:about="http://www.essepuntato.it/2012/04/tvc/withinContext"/>
    


    <!-- http://www.ontologydesignpatterns.org/cp/owl/timeindexedsituation.owl#atTime -->

    <owl:ObjectProperty rdf:about="http://www.ontologydesignpatterns.org/cp/owl/timeindexedsituation.owl#atTime">
        <rdf:type rdf:resource="http://www.w3.org/2002/07/owl#FunctionalProperty"/>
        <rdfs:comment xml:lang="en">A time interval during which a role is held or a contribution is made by an agent.</rdfs:comment>
        <rdfs:label xml:lang="en">at time</rdfs:label>
    </owl:ObjectProperty>
    


    <!-- http://www.ontologydesignpatterns.org/cp/owl/timeindexedsituation.owl#forEntity -->

    <owl:ObjectProperty rdf:about="http://www.ontologydesignpatterns.org/cp/owl/timeindexedsituation.owl#forEntity"/>
    


    <!-- http://www.ontologydesignpatterns.org/cp/owl/timeindexedsituation.owl#hasTimeIndexedSetting -->

    <owl:ObjectProperty rdf:about="http://www.ontologydesignpatterns.org/cp/owl/timeindexedsituation.owl#hasTimeIndexedSetting"/>
    


    <!-- 
    ///////////////////////////////////////////////////////////////////////////////////////
    //
    // Data properties
    //
    ///////////////////////////////////////////////////////////////////////////////////////
     -->

    


    <!-- http://www.ontologydesignpatterns.org/cp/owl/timeinterval.owl#hasIntervalDate -->

    <owl:DatatypeProperty rdf:about="http://www.ontologydesignpatterns.org/cp/owl/timeinterval.owl#hasIntervalDate"/>
    


    <!-- http://www.ontologydesignpatterns.org/cp/owl/timeinterval.owl#hasIntervalEndDate -->

    <owl:DatatypeProperty rdf:about="http://www.ontologydesignpatterns.org/cp/owl/timeinterval.owl#hasIntervalEndDate"/>
    


    <!-- http://www.ontologydesignpatterns.org/cp/owl/timeinterval.owl#hasIntervalStartDate -->

    <owl:DatatypeProperty rdf:about="http://www.ontologydesignpatterns.org/cp/owl/timeinterval.owl#hasIntervalStartDate"/>
    


    <!-- 
    ///////////////////////////////////////////////////////////////////////////////////////
    //
    // Classes
    //
    ///////////////////////////////////////////////////////////////////////////////////////
     -->

    


    <!-- http://purl.org/spar/pro/PublishingRole -->

    <owl:Class rdf:about="http://purl.org/spar/pro/PublishingRole">
        <rdfs:subClassOf rdf:resource="http://purl.org/spar/pro/Role"/>
        <rdfs:comment xml:lang="en">A role an agent may have with respect to the publishing process.  Individual members of this class are used to specify particular roles.</rdfs:comment>
        <rdfs:label xml:lang="en">publishing role</rdfs:label>
    </owl:Class>
    


    <!-- http://purl.org/spar/pro/Role -->

    <owl:Class rdf:about="http://purl.org/spar/pro/Role">
        <rdfs:subClassOf rdf:resource="http://www.w3.org/2002/07/owl#Thing"/>
        <rdfs:comment xml:lang="en">A role an agent may have.  Individual members of this class or its sub-classes are used to specify particular roles.</rdfs:comment>
        <rdfs:label xml:lang="en">role</rdfs:label>
    </owl:Class>
    


    <!-- http://purl.org/spar/pro/RoleInTime -->

    <owl:Class rdf:about="http://purl.org/spar/pro/RoleInTime">
        <rdfs:subClassOf rdf:resource="http://www.essepuntato.it/2012/04/tvc/ValueInTime"/>
        <rdfs:subClassOf>
            <owl:Restriction>
                <owl:onProperty rdf:resource="http://purl.org/spar/pro/relatesToEntity"/>
                <owl:someValuesFrom rdf:resource="http://www.w3.org/2002/07/owl#Thing"/>
            </owl:Restriction>
        </rdfs:subClassOf>
        <rdfs:subClassOf>
            <owl:Restriction>
                <owl:onProperty rdf:resource="http://purl.org/spar/pro/withRole"/>
                <owl:someValuesFrom rdf:resource="http://purl.org/spar/pro/Role"/>
            </owl:Restriction>
        </rdfs:subClassOf>
        <rdfs:subClassOf>
            <owl:Restriction>
                <owl:onProperty rdf:resource="http://www.essepuntato.it/2012/04/tvc/atTime"/>
                <owl:someValuesFrom rdf:resource="http://www.ontologydesignpatterns.org/cp/owl/timeinterval.owl#TimeInterval"/>
            </owl:Restriction>
        </rdfs:subClassOf>
        <rdfs:subClassOf>
            <owl:Restriction>
                <owl:onProperty rdf:resource="http://www.essepuntato.it/2012/04/tvc/atTime"/>
                <owl:allValuesFrom>
                    <owl:Class>
                        <owl:intersectionOf rdf:parseType="Collection">
                            <rdf:Description rdf:about="http://www.ontologydesignpatterns.org/cp/owl/timeinterval.owl#TimeInterval"/>
                            <owl:Restriction>
                                <owl:onProperty rdf:resource="http://www.ontologydesignpatterns.org/cp/owl/timeinterval.owl#hasIntervalDate"/>
                                <owl:allValuesFrom rdf:resource="http://www.w3.org/2001/XMLSchema#dateTime"/>
                            </owl:Restriction>
                        </owl:intersectionOf>
                    </owl:Class>
                </owl:allValuesFrom>
            </owl:Restriction>
        </rdfs:subClassOf>
        <rdfs:subClassOf>
            <owl:Restriction>
                <owl:onProperty rdf:resource="http://purl.org/spar/pro/isHeldBy"/>
                <owl:qualifiedCardinality rdf:datatype="http://www.w3.org/2001/XMLSchema#nonNegativeInteger">1</owl:qualifiedCardinality>
                <owl:onClass rdf:resource="http://xmlns.com/foaf/0.1/Agent"/>
            </owl:Restriction>
        </rdfs:subClassOf>
        <dc:description xml:lang="en">A role in time describes always:
- a particular role R
- a particular agent A holding R
- a particular time interval T in which A holds R (optional)
- one or more entities (e.g. a particular bibliographic entity or a specific institution) that defines a context for R held by A. (At least one contextual entity should be specified for a particular role).</dc:description>
        <rdfs:comment xml:lang="en">A particular situation that describe a role an agent may have, that can be restricted to a particular time interval.</rdfs:comment>
        <rdfs:label xml:lang="en">role in time</rdfs:label>
    </owl:Class>
    


    <!-- http://www.essepuntato.it/2012/04/tvc/ValueInTime -->

    <owl:Class rdf:about="http://www.essepuntato.it/2012/04/tvc/ValueInTime"/>
    


    <!-- http://www.ontologydesignpatterns.org/cp/owl/timeindexedsituation.owl#TimeIndexedSituation -->

    <owl:Class rdf:about="http://www.ontologydesignpatterns.org/cp/owl/timeindexedsituation.owl#TimeIndexedSituation"/>
    


    <!-- http://www.ontologydesignpatterns.org/cp/owl/timeinterval.owl#TimeInterval -->

    <owl:Class rdf:about="http://www.ontologydesignpatterns.org/cp/owl/timeinterval.owl#TimeInterval">
        <rdfs:comment xml:lang="en">Two (starting and ending) points in time that define a particular period of time.</rdfs:comment>
        <rdfs:label xml:lang="en">time interval</rdfs:label>
    </owl:Class>
    


    <!-- http://xmlns.com/foaf/0.1/Agent -->

    <owl:Class rdf:about="http://xmlns.com/foaf/0.1/Agent">
        <rdfs:comment xml:lang="en">An abstract class defining any kind of agents, such as a person, a group, an organization or a software agent.</rdfs:comment>
        <rdfs:label xml:lang="en">agent</rdfs:label>
    </owl:Class>
    


    <!-- http://xmlns.com/foaf/0.1/Document -->

    <owl:Class rdf:about="http://xmlns.com/foaf/0.1/Document">
        <rdfs:comment xml:lang="en">An abstract class defining any kinds of publishing work.</rdfs:comment>
        <rdfs:label xml:lang="en">document</rdfs:label>
    </owl:Class>
    


    <!-- 
    ///////////////////////////////////////////////////////////////////////////////////////
    //
    // Individuals
    //
    ///////////////////////////////////////////////////////////////////////////////////////
     -->

    


    <!-- http://purl.org/spar/pro/archivist -->

    <owl:NamedIndividual rdf:about="http://purl.org/spar/pro/archivist">
        <rdf:type rdf:resource="http://purl.org/spar/pro/PublishingRole"/>
        <rdfs:comment xml:lang="en">The role of a person who manages, undertakes and supervises the work of an archive.  [This term is typically used with respect to a document archive, whereas the term data curator is used with respect to a data archive.]</rdfs:comment>
        <rdfs:label xml:lang="en">archivist</rdfs:label>
    </owl:NamedIndividual>
    


    <!-- http://purl.org/spar/pro/author -->

    <owl:NamedIndividual rdf:about="http://purl.org/spar/pro/author">
        <rdf:type rdf:resource="http://purl.org/spar/pro/PublishingRole"/>
        <rdfs:comment xml:lang="en">The role a person has of authorship of some material (for example a document).</rdfs:comment>
        <rdfs:label xml:lang="en">author</rdfs:label>
    </owl:NamedIndividual>
    


    <!-- http://purl.org/spar/pro/authors-agent -->

    <owl:NamedIndividual rdf:about="http://purl.org/spar/pro/authors-agent">
        <rdf:type rdf:resource="http://purl.org/spar/pro/PublishingRole"/>
        <rdfs:comment xml:lang="en">A person who finds work for professional authors, manages their contracts, and works to advance their careers, charging their clients as fees for their services a percentage of the money made from the authors&apos; writings.</rdfs:comment>
        <rdfs:label xml:lang="en">author&apos;s agent</rdfs:label>
    </owl:NamedIndividual>
    


    <!-- http://purl.org/spar/pro/biographer -->

    <owl:NamedIndividual rdf:about="http://purl.org/spar/pro/biographer">
        <rdf:type rdf:resource="http://purl.org/spar/pro/PublishingRole"/>
        <rdfs:comment xml:lang="en">The role of an author who writes biographies.</rdfs:comment>
        <rdfs:label xml:lang="en">biographer</rdfs:label>
    </owl:NamedIndividual>
    


    <!-- http://purl.org/spar/pro/blogger -->

    <owl:NamedIndividual rdf:about="http://purl.org/spar/pro/blogger">
        <rdf:type rdf:resource="http://purl.org/spar/pro/PublishingRole"/>
        <rdfs:comment xml:lang="en">The role of an author who writes blog posts.</rdfs:comment>
        <rdfs:label xml:lang="en">blogger</rdfs:label>
    </owl:NamedIndividual>
    


    <!-- http://purl.org/spar/pro/commissioning-editor -->

    <owl:NamedIndividual rdf:about="http://purl.org/spar/pro/commissioning-editor">
        <rdf:type rdf:resource="http://purl.org/spar/pro/PublishingRole"/>
        <rdfs:comment xml:lang="en">The role of an editor who actively commissions authors to write books to be published by the publishing house for which the commissioning editor works.</rdfs:comment>
        <rdfs:label xml:lang="en">commissioning editor</rdfs:label>
    </owl:NamedIndividual>
    


    <!-- http://purl.org/spar/pro/compiler -->

    <owl:NamedIndividual rdf:about="http://purl.org/spar/pro/compiler">
        <rdf:type rdf:resource="http://purl.org/spar/pro/PublishingRole"/>
        <rdfs:comment xml:lang="en">The role an agent has of compiling a number of items into a compilation or collection.</rdfs:comment>
        <rdfs:label xml:lang="en">compiler</rdfs:label>
    </owl:NamedIndividual>
    


    <!-- http://purl.org/spar/pro/contributor -->

    <owl:NamedIndividual rdf:about="http://purl.org/spar/pro/contributor">
        <rdf:type rdf:resource="http://purl.org/spar/pro/PublishingRole"/>
        <rdfs:comment xml:lang="en">The role an agent has of contribution of some material (for example an article to a magazine).</rdfs:comment>
        <rdfs:label xml:lang="en">contributor</rdfs:label>
    </owl:NamedIndividual>
    


    <!-- http://purl.org/spar/pro/copy-editor -->

    <owl:NamedIndividual rdf:about="http://purl.org/spar/pro/copy-editor">
        <rdf:type rdf:resource="http://purl.org/spar/pro/PublishingRole"/>
        <rdfs:comment xml:lang="en">The role of an editor who undertakes alterations to the text of a document submitted for publication to improve the formatting, style and accuracy of text, or to bring the text into the house style of the publisher (e.g. Americanization of British spelling), without intentionally altering the substance or meaning of the text.</rdfs:comment>
        <rdfs:label xml:lang="en">copy editor</rdfs:label>
    </owl:NamedIndividual>
    


    <!-- http://purl.org/spar/pro/copyright-owner -->

    <owl:NamedIndividual rdf:about="http://purl.org/spar/pro/copyright-owner">
        <rdf:type rdf:resource="http://purl.org/spar/pro/PublishingRole"/>
        <rdfs:comment xml:lang="en">The role of owning the copyright to a publication, usually held by the author or by the publishing house that publishes the author&apos;s work.</rdfs:comment>
        <rdfs:label xml:lang="en">copyright owner</rdfs:label>
    </owl:NamedIndividual>
    


    <!-- http://purl.org/spar/pro/critic -->

    <owl:NamedIndividual rdf:about="http://purl.org/spar/pro/critic">
        <rdf:type rdf:resource="http://purl.org/spar/pro/PublishingRole"/>
        <rdfs:comment xml:lang="en">The role of an author who writes evaluations and criticisms of, for example, plays or other works of art.</rdfs:comment>
        <rdfs:label xml:lang="en">critic</rdfs:label>
        <rdfs:seeAlso rdf:resource="http://purl.org/spar/pro/reviewer"/>
    </owl:NamedIndividual>
    


    <!-- http://purl.org/spar/pro/deputy-editor -->

    <owl:NamedIndividual rdf:about="http://purl.org/spar/pro/deputy-editor">
        <rdf:type rdf:resource="http://purl.org/spar/pro/PublishingRole"/>
        <rdfs:comment xml:lang="en">The role of a senior editor of a publication who deputizes for the Editor-in-Chief.</rdfs:comment>
        <rdfs:label xml:lang="en">deputy editor</rdfs:label>
    </owl:NamedIndividual>
    


    <!-- http://purl.org/spar/pro/distributor -->

    <owl:NamedIndividual rdf:about="http://purl.org/spar/pro/distributor">
        <rdf:type rdf:resource="http://purl.org/spar/pro/PublishingRole"/>
        <rdfs:comment xml:lang="en">The role of a person who distributes or disseminates publications or other resources.</rdfs:comment>
        <rdfs:label xml:lang="en">distributor</rdfs:label>
    </owl:NamedIndividual>
    


    <!-- http://purl.org/spar/pro/editor -->

    <owl:NamedIndividual rdf:about="http://purl.org/spar/pro/editor">
        <rdf:type rdf:resource="http://purl.org/spar/pro/PublishingRole"/>
        <rdfs:comment xml:lang="en">The role of a person who selects and prepares for publication material created and submitted by authors, having oversight of its content, format and presentation.</rdfs:comment>
        <rdfs:label xml:lang="en">editor</rdfs:label>
    </owl:NamedIndividual>
    


    <!-- http://purl.org/spar/pro/editor-in-chief -->

    <owl:NamedIndividual rdf:about="http://purl.org/spar/pro/editor-in-chief">
        <rdf:type rdf:resource="http://purl.org/spar/pro/PublishingRole"/>
        <rdfs:comment xml:lang="en">The role of the person who has final responsibility for the editorial operations and policies for a particular publication.</rdfs:comment>
        <rdfs:label xml:lang="en">editor-in-chief</rdfs:label>
    </owl:NamedIndividual>
    


    <!-- http://purl.org/spar/pro/executive-editor -->

    <owl:NamedIndividual rdf:about="http://purl.org/spar/pro/executive-editor">
        <rdf:type rdf:resource="http://purl.org/spar/pro/PublishingRole"/>
        <rdfs:comment xml:lang="en">The role of an editor who has executive responsibility for the production of particular publication, usually acting under the authority of the Editor-in-Chief.</rdfs:comment>
        <rdfs:label xml:lang="en">executive editor</rdfs:label>
    </owl:NamedIndividual>
    


    <!-- http://purl.org/spar/pro/ghost-writer -->

    <owl:NamedIndividual rdf:about="http://purl.org/spar/pro/ghost-writer">
        <rdf:type rdf:resource="http://purl.org/spar/pro/PublishingRole"/>
        <rdfs:comment xml:lang="en">The role of a professional writer who assists an aspiring author lacking authorship skills to write a book or article for publication, for example by helping the author to create grammatically correct and lucid prose, or who writes the book on behalf of the named author, without himself/herself claiming authorship.</rdfs:comment>
        <rdfs:label xml:lang="en">ghost writer</rdfs:label>
    </owl:NamedIndividual>
    


    <!-- http://purl.org/spar/pro/guest-editor -->

    <owl:NamedIndividual rdf:about="http://purl.org/spar/pro/guest-editor">
        <rdf:type rdf:resource="http://purl.org/spar/pro/PublishingRole"/>
        <rdfs:comment xml:lang="en">The role of someone who is a guest editor, for example for a special themed issue of a journal.</rdfs:comment>
        <rdfs:label xml:lang="en">guest editor</rdfs:label>
    </owl:NamedIndividual>
    


    <!-- http://purl.org/spar/pro/illustrator -->

    <owl:NamedIndividual rdf:about="http://purl.org/spar/pro/illustrator">
        <rdf:type rdf:resource="http://purl.org/spar/pro/PublishingRole"/>
        <rdfs:comment xml:lang="en">The role of an agent that illustrates a document.</rdfs:comment>
        <rdfs:label xml:lang="en">illustrator</rdfs:label>
    </owl:NamedIndividual>
    


    <!-- http://purl.org/spar/pro/journalist -->

    <owl:NamedIndividual rdf:about="http://purl.org/spar/pro/journalist">
        <rdf:type rdf:resource="http://purl.org/spar/pro/PublishingRole"/>
        <rdfs:comment xml:lang="en">The role of an author who writes newspaper or magazine news reports or articles.</rdfs:comment>
        <rdfs:label xml:lang="en">journalist</rdfs:label>
    </owl:NamedIndividual>
    


    <!-- http://purl.org/spar/pro/librarian -->

    <owl:NamedIndividual rdf:about="http://purl.org/spar/pro/librarian">
        <rdf:type rdf:resource="http://purl.org/spar/pro/PublishingRole"/>
        <rdfs:comment xml:lang="en">The role of a person who manages, undertakes and supervises the work of a library.</rdfs:comment>
        <rdfs:label xml:lang="en">librarian</rdfs:label>
    </owl:NamedIndividual>
    


    <!-- http://purl.org/spar/pro/managing-editor -->

    <owl:NamedIndividual rdf:about="http://purl.org/spar/pro/managing-editor">
        <rdf:type rdf:resource="http://purl.org/spar/pro/PublishingRole"/>
        <rdfs:comment xml:lang="en">The role of an editor who has management responsibility for the production of particular publication, usually acting under the authority of the Executive Editor and the Editor-in-Chief.</rdfs:comment>
        <rdfs:label xml:lang="en">managing editor</rdfs:label>
    </owl:NamedIndividual>
    


    <!-- http://purl.org/spar/pro/peer-reviewer -->

    <owl:NamedIndividual rdf:about="http://purl.org/spar/pro/peer-reviewer">
        <rdf:type rdf:resource="http://purl.org/spar/pro/PublishingRole"/>
        <rdfs:comment xml:lang="en">The role of an academic peer in evaluating a manuscript submitted by an author for publication as a journal article on behalf of the journal editor, or a conference paper on behalf of the conference programme committee, and in deciding whether it is suitable for acceptance, usually subject to revisions suggested by the peer-reviewer.</rdfs:comment>
        <rdfs:label xml:lang="en">peer reviewer</rdfs:label>
        <rdfs:seeAlso rdf:resource="http://purl.org/spar/pro/reviewer"/>
    </owl:NamedIndividual>
    


    <!-- http://purl.org/spar/pro/printer -->

    <owl:NamedIndividual rdf:about="http://purl.org/spar/pro/printer">
        <rdf:type rdf:resource="http://purl.org/spar/pro/PublishingRole"/>
        <rdfs:comment xml:lang="en">The role of an agent involved in printing documents, either a company providing printing services or an individual engaged in the process of printing documents.</rdfs:comment>
        <rdfs:label xml:lang="en">printer</rdfs:label>
    </owl:NamedIndividual>
    


    <!-- http://purl.org/spar/pro/producer -->

    <owl:NamedIndividual rdf:about="http://purl.org/spar/pro/producer">
        <rdf:type rdf:resource="http://purl.org/spar/pro/PublishingRole"/>
        <rdfs:comment xml:lang="en">The role of someone who acts as a producer.</rdfs:comment>
        <rdfs:label xml:lang="en">producer</rdfs:label>
    </owl:NamedIndividual>
    


    <!-- http://purl.org/spar/pro/production-editor -->

    <owl:NamedIndividual rdf:about="http://purl.org/spar/pro/production-editor">
        <rdf:type rdf:resource="http://purl.org/spar/pro/PublishingRole"/>
        <rdfs:comment xml:lang="en">The role of an editor who takes responsibility for the passage of a document through the various stages of the publication workflow from the submitted manuscript to the final publication, including responsibility for scheduling and budget.</rdfs:comment>
        <rdfs:label xml:lang="en">production editor</rdfs:label>
    </owl:NamedIndividual>
    


    <!-- http://purl.org/spar/pro/proof-reader -->

    <owl:NamedIndividual rdf:about="http://purl.org/spar/pro/proof-reader">
        <rdf:type rdf:resource="http://purl.org/spar/pro/PublishingRole"/>
        <rdfs:comment xml:lang="en">The role of a person who reads the proofs of documents to detect any errors prior to final publication.</rdfs:comment>
        <rdfs:label xml:lang="en">proof reader</rdfs:label>
    </owl:NamedIndividual>
    


    <!-- http://purl.org/spar/pro/publisher -->

    <owl:NamedIndividual rdf:about="http://purl.org/spar/pro/publisher">
        <rdf:type rdf:resource="http://purl.org/spar/pro/PublishingRole"/>
        <rdfs:comment xml:lang="en">The role of a person or an organization that published material, or of a publisher&apos;s employee who has responsibility for such publications.</rdfs:comment>
        <rdfs:label xml:lang="en">publisher</rdfs:label>
    </owl:NamedIndividual>
    


    <!-- http://purl.org/spar/pro/reader -->

    <owl:NamedIndividual rdf:about="http://purl.org/spar/pro/reader">
        <rdf:type rdf:resource="http://purl.org/spar/pro/PublishingRole"/>
        <rdfs:comment xml:lang="en">The role of a person who reads publications.</rdfs:comment>
        <rdfs:label xml:lang="en">reader</rdfs:label>
    </owl:NamedIndividual>
    


    <!-- http://purl.org/spar/pro/reviewer -->

    <owl:NamedIndividual rdf:about="http://purl.org/spar/pro/reviewer">
        <rdf:type rdf:resource="http://purl.org/spar/pro/PublishingRole"/>
        <rdfs:comment xml:lang="en">The role of a person who subjects a publication to a written review and critical analysis of its content, scope and quality.</rdfs:comment>
        <rdfs:label xml:lang="en">reviewer</rdfs:label>
    </owl:NamedIndividual>
    


    <!-- http://purl.org/spar/pro/senior-editor -->

    <owl:NamedIndividual rdf:about="http://purl.org/spar/pro/senior-editor">
        <rdf:type rdf:resource="http://purl.org/spar/pro/PublishingRole"/>
        <rdfs:comment xml:lang="en">The role of the person who has senior responsibility for the editorial operations and policies for a particular publication, usually acting under the authority of the Editor-in-Chief.</rdfs:comment>
        <rdfs:label xml:lang="en">senior editor</rdfs:label>
    </owl:NamedIndividual>
    


    <!-- http://purl.org/spar/pro/series-editor -->

    <owl:NamedIndividual rdf:about="http://purl.org/spar/pro/series-editor">
        <rdf:type rdf:resource="http://purl.org/spar/pro/PublishingRole"/>
        <rdfs:comment xml:lang="en">The role of the person who has editorial responsibility for publication series, for example a book series.</rdfs:comment>
        <rdfs:label xml:lang="en">series editor</rdfs:label>
    </owl:NamedIndividual>
    


    <!-- http://purl.org/spar/pro/translator -->

    <owl:NamedIndividual rdf:about="http://purl.org/spar/pro/translator">
        <rdf:type rdf:resource="http://purl.org/spar/pro/PublishingRole"/>
        <rdfs:comment xml:lang="en">The role of an agent that translates a document into another language.</rdfs:comment>
        <rdfs:label xml:lang="en">translator</rdfs:label>
    </owl:NamedIndividual>
</rdf:RDF>



<!-- Generated by the OWL API (version 4.2.8.20170104-2310) https://github.com/owlcs/owlapi -->

